Preparing to play with initial marking of RD

FlowEquivalence.v
@@ -10,24 +10,23 @@ Import ListNotations.
 Open Scope list_scope.
 
 
-Inductive value := 
-| B0 : value
-| B1 : value
-| X  : value
-| Z  : value.
+Section FE.
+
+  Context (even odd : Set).
+  Context `{Heven : eq_dec even} `{Hodd : eq_dec odd}.  
+
 
 
 Section LatchSequence.
 
-  Context (even odd : Set).
   Inductive latch : Set := 
   | Odd : odd -> latch
   | Even : even -> latch
   .
   Arguments latch : clear implicits.
   Inductive event : Set :=
-  | Pos : latch -> event
-  | Neg : latch -> event
+  | Rise : latch -> event
+  | Fall : latch -> event
   . 
 
   Inductive CLK : Set := CLK0 | CLK1.
@@ -37,9 +36,7 @@ Section LatchSequence.
     | CLK1 => CLK0
     end.
 
-  Definition latch_set := latch -> bool.
-
-  Context `{Heven : eq_dec even} `{Hodd : eq_dec odd}.  
+  Definition transparency_predicate := latch -> bool.
 
   Instance latch_eq_dec : eq_dec latch.
   Proof.
@@ -65,23 +62,12 @@ Section LatchSequence.
       right. inversion 1. contradiction.
   Defined.
 
-
-  Definition event_refers_to_latch (e : event) (l : latch) : bool :=
-    match e with
-    | Pos l' => eqb l l'
-    | Neg l' => eqb l l'
-    end.
-
-  Definition event_becomes_transparent (e : event) : bool :=
-  match e with
-  | Pos _ => true
-  | Neg _  => false
-  end.
-
-  Definition step_latch_set (e : event) (t : latch_set) : latch_set :=
-    fun l => if event_refers_to_latch e l
-             then event_becomes_transparent e
-             else t l.
+  Definition update_transparency_predicate (e : event) (P : transparency_predicate) : transparency_predicate :=
+    fun l => if Rise l =? e
+             then true
+             else if Fall l =? e
+             then false
+             else P l.
 
   Definition is_even (l : latch) : bool :=
   match l with
@@ -91,26 +77,26 @@ Section LatchSequence.
   Definition is_odd (l : latch) : bool := negb (is_even l).
 
 
-  (* A latch sequence is a snoc-list of events, ending with a set of transparent latches. *)
-  Inductive latch_sequence : Set :=
-  | ls_empty_async (transparent_set : latch_set) : latch_sequence
-  | ls_async (e : event)
-             (next : latch_sequence)
-           : latch_sequence
+  (* A trace is a snoc-list of events, ending with a set of transparent latches. *)
+  Inductive trace : Set :=
+  | empty_trace (P : transparency_predicate) : trace
+  | next_trace (e : event)
+             (next : trace)
+           : trace
   .
 
   (* Calculate the set of transparent latches after executing the latch sequence s *)
-  Fixpoint is_transparent (s : latch_sequence) : latch_set :=
+  Fixpoint transparent (s : trace) : transparency_predicate :=
     match s with
-    | ls_empty_async ls  => ls
-    | ls_async e s' => step_latch_set e (is_transparent s')
+    | empty_trace ls  => ls
+    | next_trace e s' => update_transparency_predicate e (transparent s')
     end.
 
 
-  Fixpoint num_events (e : event) (s : latch_sequence) : nat :=
+  Fixpoint num_events (e : event) (s : trace) : nat :=
     match s with
-    | ls_empty_async _ => 0
-    | ls_async e' s' => if e =? e'
+    | empty_trace _ => 0
+    | next_trace e' s' => if e =? e'
                         then 1 + num_events e s'
                         else num_events e s'
     end.
@@ -118,16 +104,6 @@ Section LatchSequence.
 
 End LatchSequence.
 
-Arguments Odd {even odd}.
-Arguments Even {even odd}.
-Arguments is_transparent {even odd Heven Hodd}.
-
-Arguments ls_empty_async {even odd}.
-Arguments ls_async {even odd}.
-
-Arguments Pos {even odd}.
-Arguments Neg {even odd}.
-Arguments num_events {even odd Heven Hodd}.
 
 (*************)
 (** Circuits *)
@@ -135,16 +111,19 @@ Arguments num_events {even odd Heven Hodd}.
 
 Section Circuits.
 
-  Variable even odd : Set.
-  Context `{Heven : eq_dec even} `{Hodd : eq_dec odd}.  
+  Inductive value := 
+  | B0 : value
+  | B1 : value
+  | X  : value
+  | Z  : value.
 
   Definition state (tp : Set) := tp -> value.
 
   Definition odd_state {P : odd -> Prop}
-                       (s : state (latch even odd)) : state {o : odd & P o} :=
+                       (s : state latch) : state {o : odd & P o} :=
     fun o => s (Odd (projT1 o)).
   Definition even_state {P : even -> Prop}
-                        (s : state (latch even odd)) : state {e : even & P e} :=
+                        (s : state latch) : state {e : even & P e} :=
     fun o => s (Even (projT1 o)).
 
   Record circuit : Set :=
@@ -155,42 +134,41 @@ Section Circuits.
   }.
 
   Definition get_latch_value (c : circuit)
-                             (prev : state (latch even odd))
-                             (l : latch even odd) : value :=
+                             (prev : state latch)
+                             (l : latch) : value :=
     match l with
     | Even e => evenF c e (odd_state prev)
     | Odd o  => oddF c o (even_state prev)
     end.
 
-
   (** Async execution *)
 
   Definition state_respects_transparencies (c : circuit)
-                                        (s : latch_sequence even odd)
-                                        (st : state (latch even odd)) :=
-    forall l, is_transparent s l = true -> st l = get_latch_value c st l.
+                                           (P : transparency_predicate)
+                                           (st : state latch) :=
+    forall l, P l = true -> st l = get_latch_value c st l.
 
-  Definition state_respects_opacities (s : latch_sequence even odd)
-                                      (st1 st2 : state (latch even odd)) :=
-    forall l, is_transparent s l = false -> st1 l = st2 l.
+  Definition state_respects_opacities (P : transparency_predicate)
+                                      (st1 st2 : state latch) :=
+    forall l, P l = false -> st1 l = st2 l.
 
 
   Reserved Notation " c '⊢' st '⇒' s '⇒' st' " (no associativity, at level 80).
-  Inductive eval (c : circuit) (init : state (latch even odd))
-               : latch_sequence even odd -> state (latch even odd) -> Prop :=
-  | eval_nil lset : 
-    state_respects_transparencies c (ls_empty_async lset) init ->
-    c ⊢ init ⇒ ls_empty_async lset ⇒ init
+  Inductive eval (c : circuit) (init : state latch)
+               : trace -> state latch -> Prop :=
+  | eval_nil P : 
+    state_respects_transparencies c P init ->
+    c ⊢ init ⇒ empty_trace P ⇒ init
   | eval_cons e s st st' :
     c ⊢ init ⇒s⇒ st ->
-    state_respects_opacities (ls_async e s) st' st ->
-    state_respects_transparencies c (ls_async e s) st' ->
-    c ⊢ init ⇒ls_async e s⇒ st'
+    state_respects_opacities (transparent (next_trace e s)) st' st ->
+    state_respects_transparencies c (transparent (next_trace e s)) st' ->
+    c ⊢ init ⇒next_trace e s⇒ st'
   where " c '⊢' st '⇒' s '⇒' st' " := (eval c st s st').
 
   Lemma eval_transparent : forall c st s st',
     c ⊢ st ⇒ s ⇒ st' ->
-    forall l, is_transparent s l = true -> st' l = get_latch_value c st' l.
+    forall l, transparent s l = true -> st' l = get_latch_value c st' l.
   Proof.
     intros c st s st' H.
     induction H; intros invariant l; auto.
@@ -199,74 +177,80 @@ Section Circuits.
 
  
   (** Syncronous execution *)
-  Fixpoint sync_even (c : circuit) (st : state (latch even odd)) (n : nat)
-                            {struct n} : state even :=
-    fun E =>
-    evenF c E (fun O => match n with
-                        | 0 => st (Odd (projT1 O))
-                        | S n' => oddF c (projT1 O) (fun E => sync_even c st n' (projT1 E))
-                        end).
-  Fixpoint sync_odd (c : circuit) (st : state (latch even odd)) (n : nat) 
-                            {struct n} : state odd :=
+  Fixpoint sync_odd (c : circuit) (st : state latch) (n : nat)
+                    {struct n} : state odd. Admitted.
+(*
     fun O =>
     match n with
     | 0 => st (Odd O)
-    | S n' => oddF c O (fun E => sync_even c st n' (projT1 E))
+    | S n' => oddF c O (fun E => evenF c (projT1 E) (fun O => sync_odd c st n' (projT1 O)))
     end.
-  Lemma sync_even_eq : forall c st n E,
-    sync_even c st n E = evenF c E (fun O => sync_odd c st n (projT1 O)).
-  Proof.
-    intros.
-    induction n.
-    * simpl. reflexivity.
-    * simpl. reflexivity. 
-  Qed.
+*)
+  Fixpoint sync_even (c : circuit) (st : state latch) (n : nat) 
+                            {struct n} : state even. Admitted.
+(*
+    fun E =>
+    match n with
+    | 0 => st (Even E)
+    | S n' => evenF c E (fun O => sync_odd c st n' (projT1 O))
+    end.
+*)
 
-  Definition sync_eval (c : circuit) (st : state (latch even odd)) (n : nat) 
-                   : state (latch even odd) := fun l =>
+  Definition sync_eval (c : circuit) (st : state latch) (n : nat) 
+                   : state latch := fun l =>
     match l with
     | Even E => sync_even c st n E
     | Odd o  => sync_odd c st n o
     end.
 
-  Lemma sync_eval_even : forall (c : circuit) (st : state (latch even odd)) n E,
+
+(* NOTE: if your execution model starts with the clock going low (e.g. even first), then you would need to reverse the order of synchronous execution and derive the following results:
+*)
+
+  Lemma sync_eval_even : forall (c : circuit) (st : state latch) n E,
         sync_eval c st n (Even E) = evenF c E (odd_state (sync_eval c st n)).
-  Proof.
-    intros c st n E. simpl. 
-    rewrite sync_even_eq. reflexivity.
-  Qed.
+  Admitted.
   Lemma sync_eval_odd_0 : forall c st O,
         sync_eval c st 0 (Odd O) = st (Odd O).
-  Proof.
-    reflexivity.
-  Qed.
+  Admitted.
   Lemma sync_eval_odd : forall c st n O,
         sync_eval c st (S n) (Odd O) = oddF c O (even_state (sync_eval c st n)).
+  Admitted.
+
+
+(*
+  Lemma sync_eval_0 : forall c st O,
+        sync_eval c st 0 (Odd O) = st (Odd O).
   Proof.
-    reflexivity.
+(*
+    intros. destruct l; reflexivity.
   Qed.
-  Lemma sync_eval_even_0_opp : forall c st E,
-        sync_eval c st 0 (Even E) = st (Even E).
+*)
   Admitted.
-  Lemma sync_eval_even_opp : forall c st n E,
+
+  Lemma sync_eval_even: forall c st n E,
         sync_eval c st (S n) (Even E) = evenF c E (odd_state (sync_eval c st n)).
-  Admitted.
-  Lemma sync_eval_odd_opp : forall c st n O,
-        sync_eval c st n (Odd O) = oddF c O (even_state (sync_eval c st n)).
-  Admitted.
+  Proof.
+(*
+    intros. simpl. reflexivity.
+  Qed.
+*)
+Admitted.
+  Lemma sync_eval_odd : forall c st n O,
+        sync_eval c st (S n) (Odd O) = oddF c O (even_state (sync_eval c st (S n))).
+  Proof.
+(*
+    intros. simpl.
+    destruct n; auto.
+  Qed.
+*)
+Admitted.
+*)
+
 
 End Circuits.
 
-Arguments eval {even odd Heven Hodd}.
 Notation " c '⊢' st '⇒' s '⇒' st' " := (eval c st s st') (no associativity, at level 80).
-
-Arguments odd_even_neighbors {even odd}.
-Arguments even_odd_neighbors {even odd}.
-
-
-Class Enumerable (A : Set) :=
-  { enumerate : list A }.
-
 
 (******************)
 (** Marked graphs *)
@@ -274,125 +258,153 @@ Class Enumerable (A : Set) :=
 
 Section MarkedGraphs.
 
-  Context (events : Set).
+(*
   Context (transitions : Set).
-  Context `{Hevents : eq_dec events}.
+  Context (places : Set).
   Context `{Htransitions : eq_dec transitions}.
-(*  Context `{Enumerable transitions}. *)
+  Context `{Hplaces : eq_dec places}.
+*)
 
-  Definition marking := transitions -> nat.
+  Definition marking places := places -> nat.
 
-  Record marked_graph : Set :=
-  { input_event_output : list (events * transitions * events) }.
-  Definition input_event (M : marked_graph) : list (events * transitions) :=
+  Record marked_graph (transitions : Set) (places : Set) : Set :=
+  { input_event_output : list (transitions * places * transitions) }.
+  Arguments input_event_output {transitions places}.
+  Definition input_event {transitions places} 
+                         (M : marked_graph transitions places) : list (transitions * places) :=
     fmap fst (input_event_output M).
-  Definition output_event (M : marked_graph) : list (transitions * events) :=
+  Definition output_event {transitions places}
+                          (M : marked_graph transitions places) : list (places * transitions) :=
     fmap (fun ete => (snd (fst ete),snd ete)) (input_event_output M).
 
-  Definition in_transitions (M : marked_graph) (e : events) : list transitions :=
-    let f := fun ete => if snd ete =? e then [snd (fst ete)] else [] in
+  Definition in_places {transitions places : Set}
+                       `{eq_dec transitions}
+                       (M : marked_graph transitions places) (t : transitions) : list places :=
+    let f := fun ete => if snd ete =? t then [snd (fst ete)] else [] in
     flat_map f (input_event_output M).
 
-  Definition enabled (e : events)
-                     (M : marked_graph)
-                     (m : marking)
+  Definition enabled {transitions places : Set} `{Htransitions : eq_dec transitions}
+                     (e : transitions)
+                     (M : marked_graph transitions places)
+                     (m : marking places)
                    : bool :=
-    forallb (fun t => Nat.ltb 0 (m t)) (in_transitions M e).
-  Definition is_enabled (M : marked_graph) (e : events) (m : marking) :=
+    forallb (fun t => Nat.ltb 0 (m t)) (in_places M e).
+  Definition is_enabled {transitions places : Set}  `{Htransitions : eq_dec transitions}
+                        (M : marked_graph transitions places)
+                        (e : transitions)
+                        (m : marking places) :=
     enabled e M m = true.
 
   (* An event should only fire if the caller has independently checked that it
   is enabled. *) 
+  Definition fire {transitions places : Set}
+                  `{Htransitions : eq_dec transitions}
+                  `{Hplaces : eq_dec places}
+                  (t : transitions)
+                  (M : marked_graph transitions places)
+                  (m : marking places)
+                : marking places :=
+  fun p => if in_dec' (p,t) (output_event M) (* e0 →t→ e *)
+           then m p - 1 (* remove markings on in-edges of e *)
+           else if in_dec' (t,p) (input_event M) (* e →t→ e0 *)
+           then m p + 1 (* add marking to out-edges of e *)
+           else m p.
 
-  Definition fire (e : events)
-                  (M : marked_graph)
-                  (m : marking)
-                : marking :=
-  fun t => if in_dec' (t,e) (output_event M) (* e0 →t→ e *)
-           then m t - 1 (* remove markings on in-edges of e *)
-           else if in_dec' (e,t) (input_event M) (* e →t→ e0 *)
-           then m t + 1 (* add marking to out-edges of e *)
-           else m t.
 
 
 End MarkedGraphs.
 
-Arguments in_transitions {events transitions}.
+(*********************)
+(** Flow Equivalence *)
+(*********************)
+
+Existing Instance event_eq_dec.
 
 
-Arguments Pos {even odd}.
-Arguments Neg {even odd}.
-Arguments enabled {events transitions Hevents}.
-Arguments fire {events transitions Hevents Htransitions}.
+Section FlowEquivalence.
 
+
+  Reserved Notation "{ MG }⊢ m → s → m'" (no associativity, at level 90).
+About is_enabled.
+
+  Inductive ls_consistent_with_MG {places : Set} `{Hplaces : eq_dec places}
+                                  (M : marked_graph event places)
+                                  (init_m : marking places)
+                                : trace -> marking places -> Prop :=
+  | lsc_empty lset : 
+    (forall l, is_enabled M (Rise l) init_m -> lset l = false) ->
+    (forall l, is_enabled M (Fall l) init_m -> lset l = true) ->
+    {M}⊢ init_m →empty_trace lset→ init_m
+  | lsc_cons e m m' s' : is_enabled M e m ->
+                fire e M m = m' ->
+                {M}⊢ init_m →s'→ m ->
+                {M}⊢ init_m →next_trace e s'→ m'
+  where
+    "{ MG }⊢ m → s → m'" := (ls_consistent_with_MG MG m s m').
+
+
+  Definition flow_equivalence {places : Set} `{Hplaces : eq_dec places}
+                              (M : marked_graph event places)
+                              (init_m : marking places)
+                              (c : circuit) 
+                              (init_st : state latch) :=
+    forall (t : trace),
+        (exists m, {M}⊢ init_m →t→ m) ->
+        forall st, c ⊢ init_st ⇒ t ⇒ st ->
+        forall l, transparent t l = false ->
+                  st l = sync_eval c init_st (num_events (Fall l) t) l.
+
+
+End FlowEquivalence.
+
+End FE.
+
+Arguments flow_equivalence {even odd Heven Hodd places Hplaces}.
+(*Arguments sync_eval {even odd} c. *)
+
+Arguments ls_consistent_with_MG {even odd Heven Hodd places Hplaces}.
+Notation "{ MG }⊢ m → s → m'" := (ls_consistent_with_MG MG m s m')
+                                (no associativity, at level 90).
+
+
+Arguments Odd {even odd}.
+Arguments Even {even odd}.
+Arguments transparent {even odd Heven Hodd}.
+
+Arguments empty_trace {even odd}.
+Arguments next_trace {even odd}.
+
+Arguments Rise {even odd}.
+Arguments Fall {even odd}.
+Arguments num_events {even odd Heven Hodd}.
+
+Arguments eval {even odd Heven Hodd}.
+Notation " c '⊢' st '⇒' s '⇒' st' " := (eval c st s st') (no associativity, at level 80).
+
+Arguments odd_even_neighbors {even odd}.
+Arguments even_odd_neighbors {even odd}.
+
+Arguments Rise {even odd}.
+Arguments Fall {even odd}.
 
 Arguments get_latch_value {even odd}.
+
+
+Arguments in_places {transitions places}.
+
+
+Arguments enabled {transitions places Htransitions}.
+Arguments fire {transitions places Htransitions Hplaces}.
+
 
 Arguments oddF {even odd}.
 Arguments evenF {even odd}.
 Arguments even_state {even odd P}.
 Arguments odd_state {even odd P}.
 Arguments sync_eval {even odd}.
-Arguments is_enabled {events transitions Hevents}.
+Arguments is_enabled {transitions places Htransitions}.
+Arguments state_respects_transparencies {even odd}.
+Arguments state_respects_opacities {even odd}.
 
-
-(*********************)
-(** Flow Equivalence *)
-(*********************)
-
-
-Section FlowEquivalence.
-
-  Context (even odd : Set).
-  Context `{Heven : eq_dec even} `{Hodd : eq_dec odd}.
-
-  Context (transitions : Set).
-  Context `{Htrans : eq_dec transitions}.
-
-  Variable M : marked_graph (event even odd) transitions.
-  Variable init : marking transitions.
-
-  Existing Instance event_eq_dec.
-
-
-  (* An initial marking indicates an initial state in that for each latch l, if
-  l+ is enabled first, then l=0, and if l- is enabled first, then l=1. *)
-  Definition marking_to_state (m : marking transitions) : state (latch even odd) := 
-    fun l => if enabled (Pos l) M m then B0
-             else if enabled (Neg l) M m then B1
-             else X.
-
-  Inductive ls_consistent_with_MG : latch_sequence even odd -> marking transitions -> Prop :=
-  | lsc_empty lset : 
-    (forall l, is_enabled M (Pos l) init -> lset l = false) ->
-    (forall l, is_enabled M (Neg l) init -> lset l = true) ->
-    ls_consistent_with_MG (ls_empty_async lset) init
-  | lsc_cons e m m' s' : is_enabled M e m ->
-                fire e M m = m' ->
-                ls_consistent_with_MG s' m ->
-                ls_consistent_with_MG (ls_async e s') m'
-  .
-
-  Definition consistent (s : latch_sequence even odd) : Prop := exists m, ls_consistent_with_MG s m.
-
-
-  Definition flow_equivalence (c : circuit even odd) :=
-    forall (s : latch_sequence even odd),
-        consistent s ->
-        forall st,
-        eval c (marking_to_state init) s st ->
-        forall l, is_transparent s l = false ->
-                  st l = sync_eval c (marking_to_state init) (num_events (Neg l) s) l.
-
-
-End FlowEquivalence.
-
-
-Arguments consistent {even odd Heven Hodd transitions Htrans}.
-Arguments flow_equivalence {even odd Heven Hodd transitions Htrans}.
-Arguments marking_to_state {even odd Heven Hodd transitions}.
-Arguments sync_eval {even odd} c. 
-
-Arguments ls_consistent_with_MG {even odd Heven Hodd transitions Htrans}.
-Notation "MG ⊢ m → s → m'" := (ls_consistent_with_MG MG m s m')
-                                (no associativity, at level 90).
+Existing Instance event_eq_dec.
+ 
