RiseDecoupled.v
@@ -5,16 +5,23 @@ Open Scope list_scope.
 
 
 
+Search Nat.ltb.
+Require Import PeanoNat.
+Infix "<?" := (Nat.ltb).
+
 Existing Instance event_eq_dec.
 Existing Instance latch_eq_dec.
 
 Require Import Coq.Logic.FunctionalExtensionality.
+Import Coq.Logic.ProofIrrelevance.
+
 
 Section RiseDecoupled.
 
   Context (even odd : Set).
   Context `{Heven : eq_dec even} `{Hodd : eq_dec odd}.
   Variable c : circuit even odd.
+  Variable init_st : state (latch even odd).
 
 
   Inductive transitions_RD : Set :=
@@ -28,7 +35,6 @@ Section RiseDecoupled.
   | Odd_even_fall (A : odd)  (B : even) : In (A,B) (odd_even_neighbors c) -> transitions_RD (* A- → B- *)
   .
 
-  Import Coq.Logic.ProofIrrelevance.
 
   Instance eqdecRD : eq_dec transitions_RD.
   Proof.
@@ -50,19 +56,19 @@ Section RiseDecoupled.
            : marked_graph (event even odd) transitions_RD :=
   {| input_event_output := 
      let eo_f := fun (A : even) (B : odd) pf =>
-                     [ (Pos (Even A), Even_fall A, Neg (Even A))
-                     ; (Neg (Even A), Even_odd_fall A B pf, Neg (Odd B))
-                     ; (Neg (Odd B), Odd_even_rise A B pf, Pos (Even A))
-                     ; (Pos (Odd B), Odd_fall B, Neg (Odd B))
-                     ; (Neg (Odd B), Odd_rise B, Neg (Odd B))
+                     [ (Rise (Even A), Even_fall A, Fall (Even A))
+                     ; (Fall (Even A), Even_odd_fall A B pf, Fall (Odd B))
+                     ; (Fall (Odd B), Odd_even_rise A B pf, Rise (Even A))
+                     ; (Rise (Odd B), Odd_fall B, Fall (Odd B))
+                     ; (Fall (Odd B), Odd_rise B, Fall (Odd B))
                      ]
      in
      let oe_f := fun (A : odd) (B : even) pf =>
-                     [ (Pos (Odd A), Odd_fall A, Neg (Odd A))
-                     ; (Neg (Odd A), Odd_even_fall A B pf, Neg (Even B))
-                     ; (Neg (Even B), Even_odd_rise A B pf, Pos (Odd A))
-                     ; (Pos (Even B), Even_fall B, Neg (Even B))
-                     ; (Neg (Even B), Even_rise B, Pos (Even B))
+                     [ (Rise (Odd A), Odd_fall A, Fall (Odd A))
+                     ; (Fall (Odd A), Odd_even_fall A B pf, Fall (Even B))
+                     ; (Fall (Even B), Even_odd_rise A B pf, Rise (Odd A))
+                     ; (Rise (Even B), Even_fall B, Fall (Even B))
+                     ; (Fall (Even B), Even_rise B, Rise (Even B))
                      ]
      in flat_map_proof (even_odd_neighbors c) eo_f
      ++ flat_map_proof (odd_even_neighbors c) oe_f
@@ -77,61 +83,21 @@ Section RiseDecoupled.
              end.
 
 
-Lemma fall_enabled_transparent : forall s m l,
-    ls_consistent_with_MG rise_decoupled rise_decoupled_init s m ->
-    is_enabled rise_decoupled (Neg l) m ->
-    is_transparent s l = true.
-Admitted.
 
-Lemma rise_enabled_opaque : forall s m l,
-    ls_consistent_with_MG rise_decoupled rise_decoupled_init s m ->
-    is_enabled rise_decoupled (Pos l) m ->
-    is_transparent s l = false.
-Admitted.
-
-Lemma fall_enabled_even_opaque : forall s m O E,
-    ls_consistent_with_MG rise_decoupled rise_decoupled_init s m ->
-    is_enabled rise_decoupled (Neg (Odd O)) m ->
-    In (E,O) (even_odd_neighbors c) ->
-    is_transparent s (Even E) = false.
-Admitted.
-
-Lemma fall_enabled_odd_opaque : forall s m O E,
-    ls_consistent_with_MG rise_decoupled rise_decoupled_init s m ->
-    is_enabled rise_decoupled (Neg (Even E)) m ->
-    In (O,E) (odd_even_neighbors c) ->
-    is_transparent s (Odd O) = false.
-Admitted.
-
-Lemma fall_enabled_even_odd : forall s m O E,
-    ls_consistent_with_MG rise_decoupled rise_decoupled_init s m ->
-    is_enabled rise_decoupled (Neg (Odd O)) m ->
-    In (E,O) (even_odd_neighbors c) ->
-    num_events (Neg (Even E)) s = 1+num_events (Neg (Odd O)) s.
-Admitted.
-
-Lemma fall_enabled_odd_even : forall s m O E,
-    ls_consistent_with_MG rise_decoupled rise_decoupled_init s m ->
-    is_enabled rise_decoupled (Neg (Even E)) m ->
-    In (O,E) (odd_even_neighbors c) ->
-    num_events (Neg (Odd O)) s = num_events (Neg (Even E)) s.
-Admitted.
-
-
-Lemma rise_decoupled_init_even : forall lset E,
-    consistent rise_decoupled rise_decoupled_init (ls_empty_async lset) ->
+Lemma rise_decoupled_init_even : forall lset E m,
+    {rise_decoupled}⊢ rise_decoupled_init →empty_trace lset→ m ->
     lset (Even E) = true.
 Proof.
-  intros lset E [m Hm].
+  intros lset E m Hm.
   inversion Hm as [? Hpos Hneg | ]; subst.
   apply Hneg.
   unfold is_enabled, enabled.
   apply forallb_forall.
   intros T HT.
-          unfold in_transitions, rise_decoupled in HT. simpl in HT.
+          unfold in_places, rise_decoupled in HT. simpl in HT.
           apply in_flat_map in HT.
           destruct HT as [[[e_in t] e_out] [HT H]]. simpl in *.
-          destruct (Dec e_out (Neg (Even E))); [subst; rewrite eqb_eq in H| rewrite eqb_neq in H; auto].
+          destruct (Dec e_out (Fall (Even E))); [subst; rewrite eqb_eq in H| rewrite eqb_neq in H; auto].
           inversion H as [ | H0]; [subst | inversion H0]; clear H.
           apply in_app_or in HT.
           destruct HT as [HT | HT].
@@ -145,23 +111,176 @@ Proof.
              repeat (destruct HT as [HT | HT]; [ inversion HT; subst; auto | ]); inversion HT.
 Qed.
 
+
+Open Scope nat_scope.
+Locate "<". Print marking.
+Inductive is_enabled_RD : event even odd -> marking transitions_RD -> Prop :=
+| Even_fall_enabled E m :
+  0 < m (Even_fall E) ->
+  (forall O (pf : In (O,E) (odd_even_neighbors c)),
+          0 < m (Even_odd_rise O E pf)) ->
+  is_enabled_RD (Fall (Even E)) m
+| Even_rise_enabled E m :
+  (forall O (pf : In (O,E) (odd_even_neighbors c)),
+          0 < m (Even_rise E)) ->
+  (forall O (pf : In (E,O) (even_odd_neighbors c)),
+          0 < m  (Odd_even_rise E O pf)) ->
+  is_enabled_RD (Rise (Even E)) m
+| Odd_fall_enabled O m :
+  0 < m (Odd_fall O) ->
+  (forall E (pf : In (E,O) (even_odd_neighbors c)),
+          0%nat < m (Even_odd_fall E O pf)) ->
+  is_enabled_RD (Fall (Odd O)) m
+| Odd_rise_enabled O m :
+  (forall E (pf : In (E,O) (even_odd_neighbors c)),
+          0 < m (Odd_rise O)) ->
+  (forall E (pf : In (O,E) (odd_even_neighbors c)),
+          0 < m (Even_odd_rise O E pf)) ->
+  is_enabled_RD (Rise (Odd O)) m
+.
+Lemma RD_is_enabled_equiv : forall e m,
+    is_enabled_RD e m -> is_enabled rise_decoupled e m.
+Proof.
+  destruct e as [[E | O] | [E | O]];
+    intros m; intros H.
+  * unfold is_enabled. unfold enabled. apply forallb_forall.
+    intros T pf_in.
+    inversion H; subst.
+    apply PeanoNat.Nat.ltb_lt.
+    unfold in_places in pf_in.
+    unfold rise_decoupled in pf_in. simpl in pf_in.
+    Search In flat_map.
+    apply in_flat_map in pf_in.
+    destruct pf_in as [[[e1 T0] e2] [pf_in1 pf_in2]].
+    simpl in pf_in2.
+    destruct (Dec e2 (Rise (Odd E)));
+      [ subst; rewrite eqb_eq in pf_in2; inversion pf_in2;
+        [ subst; clear pf_in2 | contradiction]
+        | rewrite eqb_neq in pf_in2; [contradiction | assumption] ].
+    apply in_app_or in pf_in1.
+    destruct pf_in1 as [pf_in1 | pf_in1].
+    ** Search In flat_map_proof.
+       apply in_flat_map_proof' in pf_in1.
+       destruct pf_in1 as [E1 [O1 [pf1 pf]]].
+       simpl in pf.
+       destruct pf as [pf | [pf | [pf | [pf | [pf | pf]]]]];
+         try (inversion pf).
+    ** apply in_flat_map_proof' in pf_in1.
+       destruct pf_in1 as [E1 [O1 [pf1 pf]]].
+       simpl in pf.
+       destruct pf as [pf | [pf | [pf | [pf | [pf | pf]]]]];
+         try (inversion pf).
+       subst.
+       apply H2.
+(* good *)
+Admitted.
+  
+Lemma is_enabled_RD_equiv : forall e m,
+    is_enabled rise_decoupled e m ->
+    is_enabled_RD e m.
+Admitted.
+
+Lemma is_enabled_fire_neq : forall {transitions : Set} `{eq_dec transitions}
+                                   (M : marked_graph (event even odd) transitions)
+                                   m e l,
+    e <> Rise l ->
+    e <> Fall l ->
+    is_enabled M (Fall l) (fire e M m) ->
+    is_enabled M (Fall l) m.
+Proof.
+    intros transitions Htransitions M m e l Hel1 Hel2 Henabled.
+    unfold is_enabled in *.
+    unfold enabled in *.
+    
+    apply forallb_forall. intros T Hin.
+
+    assert (Hfire : Nat.ltb 0 (fire e M m T) = true).
+    { destruct (forallb_forall (fun t => Nat.ltb 0 (fire e M m t)) (in_places _ M (Fall l)))
+        as [H1 H2].
+      apply H1; auto.
+    }
+    unfold fire in Hfire.
+Admitted.    
+
+  Lemma fall_enabled_transparent : forall s m l,
+    {rise_decoupled}⊢ rise_decoupled_init →s→ m ->
+    is_enabled rise_decoupled (Fall l) m ->
+    transparent s l = true.
+  Proof.
+    intros s m l pf.
+    induction pf as [lset Htransparent Hopaque | ]; intros Henabled.
+    * simpl. apply Hopaque.
+      assumption.
+    * simpl.
+      apply is_enabled_RD_equiv in Henabled.
+      destruct l as [E | O]; inversion Henabled; subst.
+      ** unfold update_transparency_predicate.
+(*
+      destruct (event_refers_to_latch even odd e l) eqn:Hel.
+      ++ destruct e as [O | E]; auto.
+         simpl in Hel.
+         
+         +++ reflexivity.
+         
+      ++ apply IHpf.
+         subst.
+         eapply is_enabled_fire_neq; eauto.
+  Qed.
+*)
+  Admitted.
+
+Lemma rise_enabled_opaque : forall s m l,
+    ls_consistent_with_MG rise_decoupled rise_decoupled_init s m ->
+    is_enabled rise_decoupled (Rise l) m ->
+    transparent s l = false.
+Admitted.
+
+Lemma fall_enabled_even_opaque : forall s m O E,
+    ls_consistent_with_MG rise_decoupled rise_decoupled_init s m ->
+    is_enabled rise_decoupled (Fall (Odd O)) m ->
+    In (E,O) (even_odd_neighbors c) ->
+    transparent s (Even E) = false.
+Admitted.
+
+Lemma fall_enabled_odd_opaque : forall s m O E,
+    ls_consistent_with_MG rise_decoupled rise_decoupled_init s m ->
+    is_enabled rise_decoupled (Fall (Even E)) m ->
+    In (O,E) (odd_even_neighbors c) ->
+    transparent s (Odd O) = false.
+Admitted.
+
+Lemma fall_enabled_even_odd : forall s m O E,
+    ls_consistent_with_MG rise_decoupled rise_decoupled_init s m ->
+    is_enabled rise_decoupled (Fall (Odd O)) m ->
+    In (E,O) (even_odd_neighbors c) ->
+    num_events (Fall (Even E)) s = 1+num_events (Fall (Odd O)) s.
+Admitted.
+
+Lemma fall_enabled_odd_even : forall s m O E,
+    ls_consistent_with_MG rise_decoupled rise_decoupled_init s m ->
+    is_enabled rise_decoupled (Fall (Even E)) m ->
+    In (O,E) (odd_even_neighbors c) ->
+    num_events (Fall (Odd O)) s = num_events (Fall (Even E)) s.
+Admitted.
+
+
+
   Theorem rise_decoupled_flow_equivalence :
-    flow_equivalence rise_decoupled rise_decoupled_init c.
+    flow_equivalence rise_decoupled rise_decoupled_init c init_st.
   Proof.
     unfold flow_equivalence.
-    induction s as [lset | e s];
-      intros Hconsistent st Heval l Hopaque.
+    induction t as [lset | e s];
+      intros [m Hm] st Heval l Hopaque.
     * simpl. 
       inversion Heval as [lset' Htransparent | ]; subst.
 
       (* Since l is opaque in the initial rise_decoupled state, it must be odd. *)
       destruct l as [O | E].
-      + (* Odd case *) simpl. reflexivity.
+      + (* Odd case *) rewrite sync_eval_odd_0. reflexivity.
       + (* Even case *) 
       contradict Hopaque. 
-      { rewrite rise_decoupled_init_even; [inversion 1 | auto]. }
+      { erewrite rise_decoupled_init_even; [inversion 1 | eauto]. }
     * simpl.
-      inversion Hconsistent as [ m Hm];
         inversion Hm as [ | e0' m0 m0' s' Henabled Hfire Hconsistent']; subst;
         rename m0 into m.
       inversion Heval as [ | ? ? st' ? Heval' Hopaque' Htransparent']; subst.
@@ -173,80 +292,80 @@ Qed.
          Heval' : c ⊢ init_state ⇒ s ⇒ st'
        *)
     
+      unfold update_transparency_predicate in Hopaque.
       (* 1. test if e=l- *)
-      destruct (Dec (Neg l) e). 
+      destruct (Dec (Fall l) e). 
       { (* e = l-, so l is opaque in st, but transparent in st'. *)
         subst. 
         rewrite eqb_eq.
         rewrite Hopaque'.
-        2:{ simpl. unfold step_latch_set. simpl. rewrite eqb_eq. reflexivity. }
+        2:{ simpl. unfold update_transparency_predicate. simpl. rewrite eqb_eq. reflexivity. }
         rewrite (eval_transparent _ _ _ _ _ _ Heval').
-        2:{ eapply fall_enabled_transparent; eauto. }
+        2:{ eapply fall_enabled_transparent; eauto. (* LEMMA*) }
         unfold get_latch_value.
 
         destruct l as [O | E].
         ++ (* l = O *)
-           rewrite sync_eval_odd_opp; auto. (* OPPOSITE *)
+           rewrite sync_eval_odd. (* OPPOSITE *)
            apply f_equal. unfold even_state.
            apply functional_extensionality.
            intros [E H_EO].
-
-           rewrite sync_eval_even_opp; auto. (* OPPOSITE *) 
            simpl.
 
            rewrite IHs; [ |eexists; eauto | assumption |].
            2:{ eapply fall_enabled_even_opaque; eauto. (* LEMMA *) }
 
-           assert (H : num_events (Neg (Even E)) s = 1+num_events (Neg (Odd O)) s).
+           assert (H : num_events (Fall (Even E)) s = 1+num_events (Fall (Odd O)) s).
            { eapply fall_enabled_even_odd; eauto. (* LEMMA *) }
            rewrite H.
 
-           rewrite sync_eval_even_opp; [ | auto | auto]. (* OPPOSITE *)
            reflexivity.
 
          ++ (* l = E *)
-           rewrite sync_eval_even_opp; auto. (* OPPOSITE *)
+           rewrite sync_eval_even. (* OPPOSITE *)
 
            apply f_equal. unfold odd_state. apply functional_extensionality.
            intros [O H_OE].
-
-           rewrite sync_eval_odd_opp; auto. (* OPPOSITE *) 
            simpl.
 
            rewrite IHs; [ |eexists; eauto | assumption |].
            2:{ eapply fall_enabled_odd_opaque; eauto. (* LEMMA *) }
 
-           assert (H : num_events (Neg (Odd O)) s = num_events (Neg (Even E)) s).
+           assert (H : num_events (Fall (Odd O)) s = num_events (Fall (Even E)) s).
            { eapply fall_enabled_odd_even; eauto. (* LEMMA *) }
            rewrite H.
-
-           rewrite sync_eval_odd_opp; [ | auto | auto]. (* OPPOSITE *)
            reflexivity.
       } 
 
       rewrite eqb_neq; [ | assumption].
 
       (* 2. Test if e = l+ *)
-      destruct (Dec (Pos l) e).
+      destruct (Dec (Rise l) e).
       { (* e = l+, so l is not opaque in st, contradiction. *)
         contradict Hopaque.
         subst.
-        unfold step_latch_set. simpl.
+        unfold update_transparency_predicate. simpl.
         rewrite eqb_eq.
         inversion 1.
       }
 
       (* 3. e <> l+ and e <> l- *)
+(*
       assert (He : event_refers_to_latch  _ _ e l = false).
       { unfold event_refers_to_latch. 
         destruct e; rewrite eqb_neq; auto; intro; subst; intuition.
       }
-      unfold step_latch_set in Hopaque.
-      rewrite He in *.
+*)
       (* Then l is opaque in both s and (e::s) *)
+      repeat (rewrite eqb_neq in Hopaque; [ | assumption]).
+
       rewrite Hopaque'.
-      2:{ simpl. unfold step_latch_set. rewrite He. apply Hopaque. }
-      rewrite IHs; [ | eexists; eauto | auto | apply Hopaque].
+      2:{ simpl. unfold update_transparency_predicate.
+          repeat (rewrite eqb_neq; [ | assumption]).          
+          apply Hopaque.
+      }
+      rewrite IHs; [ | eexists; eauto | auto | ].
+      2:{ apply Hopaque. }
       reflexivity.
   Qed.
 
